feat: add tactic `tr_split_application` (#6)
* feat tr_split_application: add dissection of input expression

* [wip] snapshot solving inhabitedExprDummy

* [wip] snapshot tr_split_application working for simple examples

* [wip] tr_split_application: weaken proof for SummableSequence to not use equalities when not needed

* [wip] tr_split_application: set priorities for instances

* [wip] tr_split_application: clean up code in SummableSequence

* [wip] tr_split_application: add relating of function head, improve tactic ergonomics

* [wip] tr_split_application: clean up code, fix linter issues

* [wip] tr_split_application: fix tr_intro may use wrong case

TraleTest/Transfer/SummableSequence.lean
@@ -3,97 +3,41 @@ import Trale.Utils.Extend
 import Trale.Utils.Split
 import Trale.Utils.Simp
 import Trale.Utils.ParamIdent
+import Trale.Utils.Application
 
 import TraleTest.Utils.Lemmas.SummableSequence
 
+set_option trace.tr.utils false
+
 -- Code based on 'summable.v' example by Trocq Rocq plugin developers.
-
--- axiom functionRelationApplication
---   (p1 : Param10 (A -> B) (A' -> B'))
---   (p2 : Param10 A A')
---   (p3 : Param10 B B')
---   :
---   ∀ f f' (_ : p1.R f f'),
---   ∀ a a' (_ : p2.R a a'), p3.R (f a) (f' a')
-
-def forallApplication
-  {α α' : Sort _}
-  {β : α -> Sort _}
-  {β' : α' -> Sort _}
-  (p1 : Param10 α α')
-  (a : α)
-  (a' : α')
-  (aR : p1.R a a')
-  (p2 : ∀ a a' (_ : p1.R a a'), Param10 (β a) (β' a'))
-  :
-  Param10 (β a) (β' a') :=
-    by
-    tr_constructor
-
-    case R =>
-      exact (p2 a a' aR).R
-
-    case right =>
-      exact (p2 a a' aR).right
-
 
 theorem sum_nnR_add : ∀ (u v : summable), (Σ (u + v) = Σ u + Σ v) := by
   tr_by sum_xnnR_add
 
   -- We use these Params
-  let _ := paramNNR
   let _ := param_summable_seq
 
+  -- TODO: Make this work with infer_instance
+  -- We need to use `propParam` instance for `Param Prop Prop`, not the
+  -- instance defined by equality.
+  let _ : Param00 Prop Prop := propParam.forget
+
+  let eqParam : Param00 (xnnR → xnnR → Prop) (nnR → nnR → Prop) := by
+    tr_split; tr_split
+
   -- Part 1: split the foralls
-  show
-    Param10
-    (∀ (f g : seq_xnnR), Σ (f + g) = Σ f + Σ g)
-    (∀ (u v : summable), Σ (u + v) = Σ u + Σ v)
-
-
-  tr_split
-  case p1 =>
-    infer_instance
-
-  intro a a' R
-
-  tr_split
-  case p1 =>
-    infer_instance
-
-  intro b b' bR
-
-  show Param10 (Σ (a + b) = Σ a + Σ b) (Σ (a' + b') = Σ a' + Σ b')
-
-  show Param10 (Eq (Σ (a + b)) (Σ a + Σ b)) (Eq (Σ (a' + b')) (Σ a' + Σ b'))
-
-  show Param10 ((fun (x : ) => (Eq (Σ (a + b))) x) (Σ a + Σ b)) ((fun (x : _) => Eq (Σ (a' + b')) x) (Σ a' + Σ b'))
+  tr_intro a a' aR
+  tr_intro b b' bR
 
   -- Part 2: Relate rhs:  X  =  *X*
   --                            ___
   --
-  let F1 := (fun x => (Σ (a + b)) = x)
-  let A1 := (Σ a + Σ b)
+  tr_split_application c c' cR by
+    unfold extend
 
-  let F2 := (fun x => (Σ (a' + b')) = x)
-  let A2 := (Σ a' + Σ b')
-
-  -- show Param10 ((_ = .) _) ((_ = .) _)
-  show Param10 (F1 A1) (F2 A2)
-
-  apply forallApplication
-
-  case p1 =>
-    show Param10 xnnR nnR
-    infer_instance
-
-  case aR =>
-    show tr.map A2 = A1; dsimp
     show .fin (Σ a' + Σ b') = Σ a + Σ b
 
-    -- If you change this to a 'let', the `subst` won't work because it will see
-    -- it as a hypothesis instead of an equality.
-    have aF : seq_extend a' = a := tr.R_implies_map a' a R
+    have aF : seq_extend a' = a := tr.R_implies_map a' a aR
     have bF : seq_extend b' = b := tr.R_implies_map b' b bR
 
     subst aF bF
@@ -101,46 +45,18 @@ theorem sum_nnR_add : ∀ (u v : summable), (Σ (u + v) = Σ u + Σ v) := by
     repeat rw [summationHomeo]
     rw [add_xnnR_homeo]
 
-  subst F1 F2 A1 A2
-
-  simp
-  intro c c' cR
-
-  show Param10 ((_ = .) c) ((_ = .) c')
-
-  have cF := tr.R_implies_map c' c cR
-  dsimp at cF
-
-  have cF2 := tr.R_implies_map c' c cR
-  dsimp at cF2
-
-
   -- Part 3: Relate lhs:  *X*  =  X
   --                      ___
   --
-  let G1 := (@Eq xnnR . c)
-  let B1 := Σ (a + b)
-
-  let G2 := (@Eq nnR . c')
-  let B2 := Σ (a' + b')
-
-  show Param10 (G1 B1) (G2 B2)
-  apply forallApplication
-
-  case p1 =>
-    show Param10 xnnR nnR
-    infer_instance
-
-  case aR =>
-    show .fin B2 = B1
+  tr_split_application d d' dR by
+    show .fin (Σ (a' + b')) = Σ (a + b)
 
     -- If you change this to a 'let', the `subst` won't work because it will see
     -- it as a hypothesis instead of an equality.
-    have aF : seq_extend a' = a := tr.R_implies_map a' a R
+    have aF : seq_extend a' = a := tr.R_implies_map a' a aR
     have bF : seq_extend b' = b := tr.R_implies_map b' b bR
 
     subst aF bF
-    unfold B1 B2
 
     have h1 : seq_extend a'.seq + seq_extend b'.seq = seq_extend (a' + b').seq := by
       congr
@@ -148,72 +64,30 @@ theorem sum_nnR_add : ∀ (u v : summable), (Σ (u + v) = Σ u + Σ v) := by
     rw [h1]
     rw [summationHomeo]
 
-  simp
-  intro d d' dR
-
-  show Param10 (G1 d) (G2 d')
-
-  have dF := tr.R_implies_map d' d dR
-  dsimp at dF
-
-  have dF2 := tr.R_implies_map d' d dR
-  dsimp at dF2
-
   show Param10 (d = c) (d' = c')
-
 
   -- Part 4: Relate eq:  X  *=*  X
   --                        ___
   --
-  let H1 := fun (f : _ -> _ -> Sort _) => (f d c)
-  let C1 := @Eq xnnR
+  tr_split_application e e' eR by
+    dsimp [inferInstance, eqParam, Param_arrow.Map0_arrow, propParam]
 
-  let H2 := fun (f : _ -> _ -> Sort _) => (f d' c')
-  let C2 := @Eq nnR
+    intro x x' xR
+    intro y y' yR
 
-  -- This and variations do not work
-  -- show Param10 ((. _ _) _ _) ((. _ _) _ _)
-  -- show Param10 ((fun (f : _ -> _ -> Sort _) => f _ _) _) ((fun (f : _ -> _ -> Sort _) => f _ _) _)
+    show x = y → x' = y'
 
-  let eqParam : Param40 (xnnR → xnnR → Prop) (nnR → nnR → Prop) := by
-    apply Param_from_map
-    intro f x y
-    exact f (.fin x) (.fin y)
+    rw [←tr.R_implies_map x x' xR]
+    rw [←tr.R_implies_map y y' yR]
 
-  show Param10 (H1 C1) (H2 C2)
-  apply forallApplication
-
-  case p1 =>
-    show Param10 (xnnR → xnnR → Prop) (nnR → nnR → Prop)
-    infer_instance
-
-  case aR =>
-    dsimp [Param_from_map]
-    funext x y
-
-    show C1 (xnnR.fin x) (xnnR.fin y) = C2 x y
-
-    unfold C1 C2
-    show (xnnR.fin x = xnnR.fin y) = (x = y)
-    simp
-
-  simp
-  intro e e' eR
-
-  show Param10 (H1 e) (H2 e')
-
-  let eF := tr.R_implies_map e e' eR
-  dsimp at eF
-
+    exact congrArg _
 
   -- Part 5: Use relations to make the relation trivial
   --
   show Param10 (e d c) (e' d' c')
-  apply (Param_id' _).forget
-  show e d c = e' d' c'
+  dsimp [inferInstance, eqParam, Param_arrow.Map0_arrow, propParam] at eR
 
-  rw [← eF]
-  show e d c = e (xnnR.fin d') (xnnR.fin c')
+  tr_from_map
+  show e d c → e' d' c'
 
-  subst dF cF
-  congr
+  exact eR d d' dR c c' cR
