TraleTest/Utils/Lemmas/SummableSequence.lean
@@ -140,7 +140,7 @@ theorem summationHomeo (a : summable) : Σ seq_extend a.seq = .fin (Σ a) := by
     contradiction
 
 
-def paramNNR : Param42b nnR xnnR
+instance paramNNR : Param42b nnR xnnR
   := SplitInj.toParam truncate_extend
 
 def param_NNR_seq : Param40 seq_nnR seq_xnnR
@@ -150,5 +150,42 @@ def param_NNR_seq : Param40 seq_nnR seq_xnnR
 def param_summable_NNR_seq : Param40 summable seq_nnR
   := Param_from_map summable.seq
 
-def param_summable_seq : Param40 summable seq_xnnR
+instance param_summable_seq : Param40 summable seq_xnnR
   := Param_from_map (param_NNR_seq.right ∘ param_summable_NNR_seq.forget.right)
+
+-- prop1 and prop2 are related if prop1 implies prop2.
+instance (priority := high) propParam : Param2a2a Prop Prop := by
+  tr_constructor
+
+  -- R
+  · intro x y
+    exact x → y
+
+  -- 2a
+  · exact id
+  · intro a a' aR
+    subst aR
+    simp
+
+  -- 2a
+  · exact id
+  · intro a a' aR
+    subst aR
+    simp
+
+/-
+TODO: Make a Prop relation which translates types it comes across. That would
+prevent needing to show equivalence of the propositions, where in some cases
+only an implication is needed or possible.
+
+```
+let eqParam2 : Param10 (xnnR → xnnR → Prop) (nnR → nnR → Prop) := by
+  tr_split
+  case p1 => infer_instance
+
+  tr_split
+  case p1 => infer_instance
+
+  infer_instance
+```
+-/
