Trale/Utils/Application.lean
@@ -1,0 +1,597 @@
+import Trale.Core.Param
+import Trale.Utils.Extend
+import Trale.Utils.Split
+import Trale.Utils.Simp
+import Trale.Utils.ParamIdent
+import Lean.Util
+import Qq
+open Qq Lean Elab Command Tactic Term Expr Meta
+
+-- axiom functionRelationApplication
+--   (p1 : Param10 (A -> B) (A' -> B'))
+--   (p2 : Param10 A A')
+--   (p3 : Param10 B B')
+--   :
+--   ∀ f f' (_ : p1.R f f'),
+--   ∀ a a' (_ : p2.R a a'), p3.R (f a) (f' a')
+
+initialize Lean.registerTraceClass `tr.utils
+-- builtin_initialize Lean.registerTraceClass `tr_split_application
+
+-- #eval show IO Unit from do
+--   Lean.registerTraceClass `tr_split_application
+
+def forallApplication
+  {α α' : Sort _}
+  {β : α -> Sort _}
+  {β' : α' -> Sort _}
+  (p1 : Param00 α α')
+  (a : α)
+  (a' : α')
+  (aR : p1.R a a')
+  (p2 : ∀ a a' (_ : p1.R a a'), Param (β a) (β' a') cov con)
+  :
+  Param (β a) (β' a') cov con := (p2 a a' aR)
+
+elab "tr_inspect_expr" td:term : tactic =>
+  withMainContext do
+    let expr ← Tactic.elabTerm td .none
+
+    trace[tr.utils] s!"Type as expression is\n  {repr expr}"
+
+    match expr with
+    | .fvar _ =>
+      --
+      let ldecl ← getFVarLocalDecl expr
+      trace[tr.utils] s!"Fvar value is\n  {repr ldecl.value}"
+
+    | _ => return ()
+
+#check Simp.SimprocsArray
+
+elab "tr_split_application'" : tactic =>
+  -- TODO Is there a more elegant way to write the constant function?
+  Lean.withTraceNode `tr.utils (fun _ => return "tr_split_application") do
+    withMainContext do
+      let goal ← getMainGoal
+      let goalType ← getMainTarget
+
+      -- trace[tr.utils] s!"Type is {goalType}"
+      -- trace[tr.utils] s!"Type as expression is {repr goalType}"
+
+      let levelU ← mkFreshLevelMVar
+      let levelV ← mkFreshLevelMVar
+      let levelW ← mkFreshLevelMVar
+
+      let fromType : Q(Sort $levelU) ← mkFreshExprMVar .none (userName := `fromType)
+      let toType : Q(Sort $levelV) ← mkFreshExprMVar .none (userName := `toType)
+
+      let covMapType : Q(MapType) ← mkFreshExprMVar (.some q(MapType)) (userName := `covMapType)
+      let conMapType : Q(MapType) ← mkFreshExprMVar (.some q(MapType)) (userName := `conMapType)
+
+      let matcher : Q(Type (max levelU levelV levelW)) := q(Param $fromType $toType $covMapType $conMapType)
+
+      if !(← isExprDefEq matcher goalType) then
+        throwTacticEx `tr_split_application goal ("goal should be of type Param")
+
+      let fromType : Q(Sort $levelU) ← instantiateMVars fromType
+      let toType : Q(Sort $levelV) ← instantiateMVars toType
+      let covMapType : Q(MapType) ← instantiateMVars covMapType
+      let conMapType : Q(MapType) ← instantiateMVars conMapType
+
+      trace[tr.utils] s!"fromType: {fromType}"
+      trace[tr.utils] s!"toType: {toType}"
+      trace[tr.utils] s!"covMap: {covMapType}"
+      trace[tr.utils] s!"conMap: {conMapType}"
+
+      let rec findFirstNonFvars
+        (fromType toType : (Expr × List Expr))
+        : MetaM ((Expr × Option Expr × List Expr) × (Expr × Option Expr × List Expr)) := do
+        let (fromType, fromArgs) := fromType
+        let (toType, toArgs) := toType
+
+        let depth := fromArgs.length
+        let pref := s!"({depth}) "
+
+        match fromType, toType with
+        | .app f a, .app g b =>
+          match a, b with
+          | .fvar _, .fvar _ =>
+            trace[tr.utils] s!"{pref}Both final arguments are fvars"
+            findFirstNonFvars
+              (f, a :: fromArgs)
+              (g, b :: toArgs)
+
+          | _, _ =>
+            match a, b with
+            | .fvar _, _
+            | _, .fvar _ =>
+              trace[tr.utils] s!"{pref}One of the final arguments is not an fvar"
+            | _, _ =>
+              trace[tr.utils] s!"{pref}Final arguments are not fvar"
+
+            -- trace[tr.utils] s!"{pref}a: {a}"
+            -- trace[tr.utils] s!"{pref}b: {b}"
+
+            -- let aDecl := LocalContext.findFVar? lctx a
+            -- let bDecl := LocalContext.findFVar? lctx b
+
+            -- trace[tr.utils] s!"{pref}aDecl: {aDecl.isSome}"
+            -- trace[tr.utils] s!"{pref}bDecl: {bDecl.isSome}"
+
+            let aType ← inferType a
+            let bType ← inferType b
+
+            -- match aDecl, bDecl with
+            -- | .some aDecl, .some bDecl =>
+            --   let aType := aDecl.type
+            --   let bType := bDecl.type
+
+            --   trace[tr.utils] s!"{pref}Type of a: {format aType}"
+            --   trace[tr.utils] s!"{pref}Type of b: {format bType}"
+
+
+            if Expr.isSort aType || Expr.isSort bType then
+              trace[tr.utils] s!"{pref}One or both types are Sort type. Skipping to next"
+              return (← findFirstNonFvars
+                (f, a :: fromArgs)
+                (g, b :: toArgs))
+
+            -- | _, _ => pure ()
+
+
+            return (
+              (f, .some a, fromArgs),
+              (g, .some b, toArgs),
+            )
+        | _, _ =>
+          trace[tr.utils] s!"{pref}No application"
+          return (
+              (fromType, .none, fromArgs),
+              (toType, .none, toArgs),
+            )
+
+      let rec sealLambda
+        (e : Expr) (count : Nat) (exampleValues : List Expr) : MetaM (Expr × List Expr) := do
+        trace[tr.utils] s!"Doing sealLambda for count {count}, (exampleValues.length: {exampleValues.length})"
+        if count > 0 then
+          throwError "Disabled sealLambda for testing"
+        match count, exampleValues with
+        | 0, _
+        | _, [] => return (e, exampleValues)
+        | n+1, a::as =>
+            let (body, remaining) ← sealLambda e n as
+            return (Expr.lam Name.anonymous (← inferType a) body BinderInfo.default, remaining)
+
+      let rec hoistFVarsToLambda'
+        (e1 e2 : Expr)
+        -- (lambdaDepth : Nat)
+        -- (isTrailing : Bool)
+        (needsSeal : Bool)
+
+        : MetaM ((Expr × List Expr) × (Expr × List Expr) × Nat) := do
+        match e1, e2 with
+        | .app f a, .app g b =>
+          trace[tr.utils] s!"[hoistFVarsToLambda'] f: {repr f}"
+          trace[tr.utils] s!"[hoistFVarsToLambda'] a: {repr a}"
+
+          match a, b with
+            | .fvar _, .fvar _ =>
+              let ((f, fVars), (g, gVars), sealDepth) ← hoistFVarsToLambda' f g needsSeal
+              return match needsSeal with
+              | true =>  (
+                  (.app f (.bvar sealDepth), a::fVars),
+                  (.app g (.bvar sealDepth), b::gVars),
+                  sealDepth + 1
+                )
+              | false => (
+                  (f, a::fVars),
+                  (g, b::gVars),
+                  0
+                )
+
+            | _, _ =>
+              let ((f, fVars), (g, gVars), sealDepth) ← hoistFVarsToLambda' f g true
+              let (fSealed, _) ← sealLambda (.app f a) sealDepth fVars
+              let (gSealed, _) ← sealLambda (.app g b) sealDepth gVars
+              return ((fSealed, fVars), (gSealed, gVars), 0)
+              -- match isTrailing with
+              -- | true => ((f, fVars), (g, gVars))
+              -- | false => ((.app f a, fVars), (.app g b, gVars))
+        | _, _ =>
+          return ((e1, []), (e2, []), 0)
+
+      -- Can't proof easily because it uses the MetaM now
+      -- have sealDepthIsZeroWhenNoSeal : ∀ e1 e2, (←hoistFVarsToLambda' e1 e2 false).3 == 0 := by
+
+      let hoistFVarsToLambda (e1 e2 : Expr) : MetaM ((Expr × Expr) × (Expr × Expr)) := do
+        let ((a1, a1Vars), (a2, a2Vars), _) ← hoistFVarsToLambda' e1 e2 false
+
+        -- let a1VarsTypes ← List.mapM inferType a1Vars
+        -- let a2VarsTypes ← List.mapM inferType a2Vars
+
+        -- let rec mkApplierFun (types : List Expr) : Expr :=
+
+        -- let applierFun1 := a1VarsTypes.foldr
+        --   (fun x y => Expr.lam .anonymous x y .default)
+        --   (.bvar 0)
+
+        trace[tr.utils] s!"[hoistFVarsToLambda] a1: {a1}"
+        trace[tr.utils] s!"[hoistFVarsToLambda] a1 repr: {repr a1}"
+        trace[tr.utils] s!"[hoistFVarsToLambda] a1Vars: {a1Vars}"
+
+        let applierFun1 := Expr.lam .anonymous (← inferType a1) (mkAppN (.bvar 0) ⟨a1Vars.reverse⟩) .default
+        -- let applierFun2 ← withLocalDeclD .anonymous (← inferType a2) (pure $ mkAppN . ⟨a2Vars⟩)
+        let applierFun2 := Expr.lam .anonymous (← inferType a2) (mkAppN (.bvar 0) ⟨a2Vars.reverse⟩) .default
+
+        trace[tr.utils] s!"[hoistFVarsToLambda] applierFun1 repr: {repr applierFun1}"
+        trace[tr.utils] s!"[hoistFVarsToLambda] applierFun1: {applierFun1}"
+
+
+        return ((applierFun1, a1), (applierFun2, a2))
+
+
+      let mut ((body1, target1, args1), (body2, target2, args2))
+        ← findFirstNonFvars (fromType, []) (toType, [])
+
+      let (a, a') ← match target1, target2 with
+      | .none, _
+      | _, .none =>
+
+        let ((f1, a1), (f2, a2)) ← hoistFVarsToLambda fromType toType
+
+        body1 ← instantiateMVars f1
+        body2 ← instantiateMVars f2
+        args1 := []
+        args2 := []
+
+        pure (← instantiateMVars a1, ← instantiateMVars a2)
+
+        -- throwTacticEx `tr_split_application goal "Can't split application: not an application, or no non-fvar arguments"
+      | some a, some a' => pure (a, a')
+
+
+      -- if target1.isNone || target2.isNone then
+      --   throwTacticEx `tr_split_application goal "Can't split application: not an application, or no non-fvar arguments"
+
+      let levelX1 ← mkFreshLevelMVar
+      let levelX2 ← mkFreshLevelMVar
+      let levelY1 ← mkFreshLevelMVar
+      let levelY2 ← mkFreshLevelMVar
+      let levelZ ← mkFreshLevelMVar
+
+
+      let α : Q(Sort $levelX1) ← inferType a
+      let α' : Q(Sort $levelX2) ← inferType a'
+      -- let α : Q(Sort $levelX1) ← mkFreshExprMVar (.some q(Sort $levelX1)) (userName := `α)
+      -- let α' : Q(Sort $levelX2) ← mkFreshExprMVar (.some q(Sort $levelX2)) (userName := `α')
+
+      -- let a : Q($α) := a
+      -- let a' : Q($α') := a'
+
+
+      -- let targetFVar1 ← mkFreshFVarId
+      -- let targetFVar2 ← mkFreshFVarId
+
+      -- let abc : LocalDecl := sorry
+      -- let ghi := abc.toExpr
+
+      -- trace[tr.utils] s!"Getting type of fvar1 and fvar2:"
+      -- -- trace[tr.utils] s!"targetFVar1: {←targetFVar1.findDecl}"
+      -- trace[tr.utils] s!"targetFVar2: {Option.map LocalDecl.toExpr (←targetFVar2.findDecl?)}"
+
+      -- let lambda1pre := mkAppN body1 ⟨(.fvar targetFVar1)::args1⟩
+
+      -- trace[tr.utils] s!"lambda1pre: {repr lambda1pre}"
+      -- let lambda1pre <- instantiateMVars lambda1pre
+
+      -- trace[tr.utils] s!"lambda1pre: {repr lambda1pre}"
+
+      -- let lambda1 ←
+      --   mkLambdaFVars #[.fvar targetFVar1]
+      --   <| lambda1pre
+
+      -- let lambda2 ← instantiateMVars <| (← mkLambdaFVars #[.fvar targetFVar2]
+      --   <| mkAppN body2 ⟨(.fvar targetFVar2)::args2⟩)
+
+      /-
+      Lean.Expr.lam
+      Lean.Name.anonymous
+      (Lean.Expr.const `_inhabitedExprDummy [])
+      (Lean.Expr.app
+
+      -/
+
+      -- let levelA1 ← mkFreshLevelMVar
+      -- let levelA2 ← mkFreshLevelMVar
+
+
+      if !(← isDefEq (← inferType α) q(Sort $levelX1)) then
+        throwTacticEx `tr_split_application goal "Failed to infer universe level of target1Type"
+
+      if !(← isDefEq (← inferType α') q(Sort $levelX2)) then
+        throwTacticEx `tr_split_application goal "Failed to infer universe level of target2Type"
+
+
+
+      let β
+          -- : Q($target1Type → $fromType)
+          : Q($α → Sort $levelY1)
+          ← withLocalDeclD `trtarget α
+          fun b => mkLambdaFVars #[b] <| mkAppN body1 ⟨b::args1⟩
+
+      let β'
+          -- : Q($target2Type → $toType)
+          : Q($α' → Sort $levelY2)
+          ← withLocalDeclD `trtarget α'
+          fun b => mkLambdaFVars #[b] <| mkAppN body2 ⟨b::args2⟩
+
+      -- trace[tr.utils] s!"lambda1 (a): {repr lambda1}"
+      -- let lambda1 ← instantiateMVars lambda1
+      -- trace[tr.utils] s!"lambda1 (b): {repr lambda1}"
+
+      let result1 : Q(Sort $levelU) := .app β a
+      let result2 : Q(Sort $levelV) := .app β' a'
+
+      -- trace[tr.utils] s!"Got result {result}"
+      let resultType : Q(Type (max levelU levelV levelW))
+        := q(Param $result1 $result2 $covMapType $conMapType)
+
+      -- evalTactic (← `(tactic| show $resultType))
+
+      if !(← isDefEq goalType resultType) then
+        throwTypeMismatchError none goalType resultType (mkStrLit "dummy")
+
+        throwTacticEx `tr_split_application goal "Failed to replace goal with new one"
+
+      -- let lambda1 : Expr ← instantiateMVars lambda1
+      -- let lambda2 : Expr ← instantiateMVars lambda2
+
+      -- trace[tr.utils] s!"α: {repr α}"
+      -- trace[tr.utils] s!"α': {repr α'}"
+      -- trace[tr.utils] s!"a: {repr a}"
+      -- trace[tr.utils] s!"lambda1: {repr β}"
+      -- trace[tr.utils] s!"lambda2: {repr β'}"
+      -- trace[tr.utils] s!"target1: {repr target1}"
+      -- trace[tr.utils] s!"target2: {repr target2}"
+
+      /-
+      The following does not work, because following it with apply or refine undoes
+      our works, eta reducing to the original goal:
+      ```
+      let newGoal ← goal.replaceTargetDefEq resultType
+      replaceMainGoal [newGoal]
+      ```
+      -/
+
+      -- let α : Q(Sort $levelU) ← mkFreshExprMVar (.some q(Sort)) (userName := `α)
+      -- let α' : Q(Sort $levelV) ← mkFreshExprMVar (.some q(Sort)) (userName := `α')
+
+      -- let α ← inferType target1
+      -- let α' ← inferType target2
+
+      -- let levelAA1 ← mkFreshLevelMVar
+      -- let levelAA2 ← mkFreshLevelMVar
+
+      -- let α : Q(Sort $levelX1) ← mkFreshExprMVar .none (userName := `α)
+      -- let α' : Q(Sort $levelX2) ← mkFreshExprMVar .none (userName := `α')
+
+      -- if !(← isExprDefEq α (←inferType target1)) then
+      --   throwTacticEx `tr_split_application goal "Failed to match type of target1 with α"
+
+      -- if !(← isExprDefEq α' (←inferType target2)) then
+      --   throwTacticEx `tr_split_application goal "Failed to match type of target2 with α"
+
+      let βType := q($α → Sort $levelY1)
+      let βType' := q($α' → Sort $levelY2)
+
+      if !(← isExprDefEq βType (←inferType β)) then
+        throwTacticEx `tr_split_application goal "Failed to match type of lambda1 with type of β"
+      if !(← isExprDefEq βType' (←inferType β')) then
+        throwTacticEx `tr_split_application goal "Failed to match type of lambda2 with type of β'"
+
+      -- let β : Q($α → Sort $levelY1) := lambda1
+      -- let β' : Q($α' → Sort $levelY2) := lambda2
+
+      -- let β : Q($α → Sort $levelY1) := sorry
+      -- let β' : Q($α' → Sort $levelY2) := sorry
+
+      /-
+      stuck at solving universe constraint
+        max
+        (max (max (max (max levelX1 levelX2) (levelY1+1)) (levelY2+1)) ?u.20766)
+        (?u.20772+1) =?= max (max levelU levelV) (levelW+1)
+      while trying to unify
+        Sort
+          (max (max (max (max (max levelX1 levelX2) ?u.20766) (levelY2 + 1)) (levelY1 + 1))
+              (?u.20772 +
+                  1)) : Type (max (max (max (max (max levelX1 levelX2) ?u.20766) (levelY2 + 1)) (levelY1 + 1)) (?u.20772 + 1))
+      with
+        Sort (max levelU levelV (levelW + 1)) : Type (max levelU levelV (levelW + 1))
+      -/
+
+      -- This does not work
+      -- let p1Type : Q(Type (max levelX1 levelX2)) := q(Param10 $α $α')
+      -- let p1 : Q($p1Type) ← mkFreshExprMVar (.some p1Type) (userName := `p1)
+
+      -- Cryptic errors like "unknown constant '_inhabitedExprDummy'"
+      --   Solved now.  Was using an fresh FVar without `withLocalDec`
+
+      -- This will be a goal
+      let p1 : Q(Param00 $α $α' : Type (max levelX1 levelX2 levelZ)) ←
+        mkFreshExprMVar (.some q((Param00 $α $α' : Type (max levelX1 levelX2 levelZ)))) (userName := `p1)
+
+      -- This will be inferred
+      -- let a : Q($α) := target1
+      -- let a' : Q($α') := target2
+      -- let a : Q($α) ← mkFreshExprMVar (.some q($α)) (userName := `a)
+      -- let a' : Q($α') ← mkFreshExprMVar (.some q($α')) (userName := `a')
+
+      /-
+      Sometimes it's a hunt for loose universe levels, and trying various things
+      until something works.
+
+      stuck at solving universe constraint
+        max
+        (max (max (max levelX1 levelX2) (levelY1+1)) (levelY2+1))
+        (?u.20373+1) =?= max (max (max levelX1 levelX2) (levelY1+1)) (levelY2+1)
+      while trying to unify
+        Sort
+          (max (max (max (max levelX1 levelX2) (levelY2 + 1)) (levelY1 + 1))
+              (?u.20373 + 1)) : Type (max (max (max (max levelX1 levelX2) (levelY2 + 1)) (levelY1 + 1)) (?u.20373 + 1))
+      with
+        Sort (max levelX1 levelX2 (levelY2 + 1) (levelY1 + 1)) : Type (max levelX1 levelX2 (levelY2 + 1) (levelY1 + 1))
+
+      -/
+      /-
+      stuck at solving universe constraint
+        max
+        (max (max (max (max levelX1 levelX2) (levelY1+1)) (levelY2+1)) levelZ)
+        (?u.20294+1) =?= max (max (max (max levelX1 levelX2) (levelY1+1)) (levelY2+1)) levelZ
+      while trying to unify
+        Sort
+          (max (max (max (max (max levelX1 levelX2) levelZ) (levelY2 + 1)) (levelY1 + 1))
+              (?u.20294 +
+                  1)) : Type (max (max (max (max (max levelX1 levelX2) levelZ) (levelY2 + 1)) (levelY1 + 1)) (?u.20294 + 1))
+      with
+        Sort
+          (max levelX1 levelX2 levelZ (levelY2 + 1)
+              (levelY1 + 1)) : Type (max levelX1 levelX2 levelZ (levelY2 + 1) (levelY1 + 1))
+      -/
+      -- let mytest
+      -- --  : Q(Sort (max levelX1 levelX2 levelZ (levelY2+1) (levelY1+1) ))
+      -- -- := q(Param10 ($β $a) ($β' $a') : Type (max (max levelX1 levelY1) (max levelX2 levelY2) levelZ))
+      -- := q(Param10 ($β $a) ($β' $a') : Type (max levelY1 levelY2 levelZ))
+
+      -- let p2Type
+      -- : Q(Sort (max levelX1 levelX2 levelZ (levelY2+1) (levelY1+1) ))
+      -- := q(∀ a a' (_ : ($p1).R a a'), (Param10 ($β a) ($β' a') : Type (max (max levelX1 levelY1) (max levelX2 levelY2) levelZ)))
+
+      let p2Type
+        : Q(Sort (max levelX1 levelX2 levelZ (levelY2+1) (levelY1+1) (levelZ+1)))
+        := q(
+            ∀ (a : $α) (a' : $α') (_ : ($p1).R a a'),
+            (Param ($β a) ($β' a') $covMapType $conMapType : Type (max levelY1 levelY2 levelZ)))
+
+      -- trace[tr.utils] s!"p2Type: {repr p2Type}"
+
+      let p2 : Q(∀ (a : $α) (a' : $α') (_: ($p1).R a a'),
+        (Param ($β a) ($β' a')  $covMapType $conMapType : Type (max levelY1 levelY2 levelZ)))
+        ← mkFreshExprMVar (.some p2Type) (userName := `p2)
+
+      -- trace[tr.utils] s!"p2: {repr p2}"
+
+      let a : Q($α) := a
+      let a' : Q($α') := a'
+
+      let aRtype := q(($p1).R $a $a')
+      -- trace[tr.utils] s!"aRtype: {repr aRtype}"
+
+      -- These will be goals
+      let aR
+        -- : Q(($p1).R $a $a')
+        ← mkFreshExprMVar (.some q(($p1).R $a $a')) (userName := `aR)
+
+      let sometest2 := q(4)
+
+      -- -- (a : α)
+      -- -- (a' : α')
+      -- -- (aR : p1.R a a')
+      -- -- (p2 : ∀ a a' (_ : p1.R a a'), Param10 (β a) (β' a'))
+
+      -- /-
+      --   {α α' : Sort _}
+      --   {β : α -> Sort _}
+      --   {β' : α' -> Sort _}
+      --   (p1 : Param10 α α')
+      --   (a : α)
+      --   (a' : α')
+      --   (aR : p1.R a a')
+      --   (p2 : ∀ a a' (_ : p1.R a a'), Param10 (β a) (β' a'))
+      --   :
+      --   Param10 (β a) (β' a')
+      -- -/
+
+
+      -- let complete := q(forallApplication $p1 $a $a' $aR $p2)
+      -- let complete := q(@forallApplication _ _ $β $β' $p1 $a $a' $aR $p2)
+      -- let almostComplete := q(fun aR => @forallApplication $covMapType $conMapType _ _ $β $β' $p1 $a $a' aR $p2)
+      let almostComplete := q(fun aR => @forallApplication $covMapType $conMapType _ _ $β $β' $p1 $a $a' aR $p2)
+      let complete : Expr := .app almostComplete aR
+
+      let completeResult : Simp.Result ← unfold complete ``forallApplication
+      let complete := completeResult.expr
+
+      -- The function `mkSimpContext`
+      let (complete, simpStats) ←
+        dsimp complete
+          (← Simp.mkContext)
+          -- (simprocs := #[{}])
+          -- (simprocs := #[←Simp.Simprocs.add {} ``forallApplication false])
+
+      -- trace[tr.utils] s!"Complete is {repr complete}"
+      -- trace[tr.utils] s!"Complete is {← ppTerm <| ← PrettyPrinter.delab complete}"
+      let complete ← instantiateMVars complete
+
+      trace[tr.utils] s!"Goal type is {format goalType}"
+
+      trace[tr.utils] s!"Complete type is {format (← inferType complete)}"
+
+      if !(← isDefEq goalType (← inferType complete)) then
+        throwTacticEx `tr_split_application goal "Could not unify goal type (1) with assembled type"
+
+      if !(← isDefEq (← goal.getType) (← inferType complete)) then
+        throwTacticEx `tr_split_application goal "Could not unify goal type (2) with assembled type"
+
+
+      trace[tr.utils] s!"Complete is {format complete}"
+
+      /-
+      While recommended by MVarId.assign, this throws, even though the above
+      type check.
+      ```
+      if !(← isDefEq (mkMVar goal) complete) then
+         throwTacticEx `tr_split_application goal "Could not unify goal with assembled value (but succeeded at type)"
+      ```
+      -/
+
+      goal.assign complete
+
+      replaceMainGoal [p1.mvarId!, aR.mvarId!, p2.mvarId!]
+
+
+
+      -- let somtest := q(4)
+      -- let complete : Q(Nat) := q(4 : Nat)
+
+
+
+      -- match fromType, toType with
+      -- | .app f a, .app g b =>
+      --   match a, b with
+      --   | .fvar _, .fvar _ =>
+      --     trace[tr.utils] s!"Both final arguments are fvars"
+      --   | .fvar _, _
+      --   | _, .fvar _ =>
+      --     trace[tr.utils] s!"One of the final arguments is not an fvar"
+      --   | _, _ =>
+      --     trace[tr.utils] s!"Final arguments are not fvar"
+      -- | _, _ =>
+      --   trace[tr.utils] s!"No application"
+
+      -- getForallArity
+
+macro "tr_split_application" : tactic => `(tactic|tr_split_application' <;> try infer_instance)
+macro "tr_split_application" ppSpace colGt a:ident a':ident aR:ident : tactic => `(
+  tactic| (
+    (tr_split_application' <;> try infer_instance); (
+      try (
+        (case' p2 => intro $a $a' $aR);rotate_left 1); tr_whnf
+        -- tr_simp_R at aR
+      )
+    )
+  )
+macro "tr_split_application" ppSpace colGt a:ident a':ident aR:ident "by" sub:tacticSeq : tactic => `(
+  tactic| (
+    (tr_split_application $a $a' $aR; case aR => $sub)
+  ))
