TraleTest/Transfer/SummableSequence_v2.lean
@@ -1,0 +1,314 @@
+import Trale.Core.Param
+import Trale.Utils.Extend
+import Trale.Utils.Split
+import Trale.Utils.Simp
+import Trale.Utils.ParamIdent
+import Trale.Utils.Application
+
+import TraleTest.Utils.Lemmas.SummableSequence
+
+set_option trace.tr.utils false
+
+-- Code based on 'summable.v' example by Trocq Rocq plugin developers.
+
+theorem sum_nnR_add : ∀ (u v : summable), (Σ (u + v) = Σ u + Σ v) := by
+  tr_by sum_xnnR_add
+
+  -- We use these Params
+  let _ := paramNNR
+  let _ := param_summable_seq
+
+  -- Part 1: split the foralls
+  show
+    Param10
+    (∀ (f g : seq_xnnR), Σ (f + g) = Σ f + Σ g)
+    (∀ (u v : summable), Σ (u + v) = Σ u + Σ v)
+
+
+  tr_split'
+  case p1 =>
+    infer_instance
+
+  intro a a' R
+
+  tr_split'
+  case p1 =>
+    infer_instance
+
+  intro b b' bR
+
+  show Param10 (Σ (a + b) = Σ a + Σ b) (Σ (a' + b') = Σ a' + Σ b')
+
+  show Param10 (Eq (Σ (a + b)) (Σ a + Σ b)) (Eq (Σ (a' + b')) (Σ a' + Σ b'))
+
+  show Param10 ((fun (x : ) => (Eq (Σ (a + b))) x) (Σ a + Σ b)) ((fun (x : _) => Eq (Σ (a' + b')) x) (Σ a' + Σ b'))
+
+  -- Part 2: Relate rhs:  X  =  *X*
+  --                            ___
+  --
+  -- let F1 := (fun x => (Σ (a + b)) = x)
+  -- let A1 := (Σ a + Σ b)
+
+  -- let F2 := (fun x => (Σ (a' + b')) = x)
+  -- let A2 := (Σ a' + Σ b')
+
+  -- show Param10 ((_ = .) _) ((_ = .) _)
+  -- show Param10 (F1 A1) (F2 A2)
+
+  tr_split_application'
+
+  -- apply forallApplication
+
+  case p1 =>
+    show Param00 xnnR nnR
+    infer_instance
+
+  case aR =>
+    -- show tr.map A2 = A1; dsimp
+    show .fin (Σ a' + Σ b') = Σ a + Σ b
+
+    -- If you change this to a 'let', the `subst` won't work because it will see
+    -- it as a hypothesis instead of an equality.
+    have aF : seq_extend a' = a := tr.R_implies_map a' a R
+    have bF : seq_extend b' = b := tr.R_implies_map b' b bR
+
+    subst aF bF
+
+    repeat rw [summationHomeo]
+    rw [add_xnnR_homeo]
+
+  -- subst F1 F2 A1 A2
+
+  simp
+  intro c c' cR
+
+  -- tr_split_application
+  /-
+  (0) Both final arguments are fvars
+  (1) Final arguments are not fvar
+  Got result (
+    (
+      Eq.{1} xnnR,
+      (
+        (
+          some (SequenceSummation.sum.{0, 0} seq_xnnR xnnR
+          instSequenceSummationSeq_xnnRXnnR (HAdd.hAdd.{0, 0, 0} seq_xnnR seq_xnnR
+          seq_xnnR (instHAdd.{0} seq_xnnR instAddSeq_xnnR) _uniq.1344 _uniq.2306))
+        ),
+        [_uniq.4944]
+      )
+    ),
+    (
+      Eq.{1} nnR,
+      (
+        (
+          some (SequenceSummation.sum.{0, 0} summable nnR instSummationSummable
+          (HAdd.hAdd.{0, 0, 0} summable summable summable (instHAdd.{0} summable
+          instAddSummable) _uniq.1347 _uniq.2309))
+        ),
+        [_uniq.4947]
+      )
+    )
+  )
+  -/
+
+  -- show Param10 ((_ = .) c) ((_ = .) c')
+
+  have cF := tr.R_implies_map c' c cR
+  dsimp at cF
+
+  have cF2 := tr.R_implies_map c' c cR
+  dsimp at cF2
+
+  -- Part 3: Relate lhs:  *X*  =  X
+  --                      ___
+  --
+  let G1 := (@Eq xnnR . c)
+  let B1 := Σ (a + b)
+
+  let G2 := (@Eq nnR . c')
+  let B2 := Σ (a' + b')
+  -- show Param10 (G1 B1) (G2 B2)
+  tr_split_application'
+
+  run_tac do
+    trace[tr.utils] "Hello"
+
+
+  -- apply forallApplication
+  -- refine' forallApplication ?_ ?_ ?_ ?_ ?_
+
+  case p1 =>
+    show Param00 xnnR nnR
+    infer_instance
+
+  case aR =>
+
+    show .fin (Σ (a' + b')) = Σ (a + b)
+    -- show .fin B2 = B1
+
+    -- If you change this to a 'let', the `subst` won't work because it will see
+    -- it as a hypothesis instead of an equality.
+    have aF : seq_extend a' = a := tr.R_implies_map a' a R
+    have bF : seq_extend b' = b := tr.R_implies_map b' b bR
+
+    subst aF bF
+    -- unfold B1 B2
+
+    have h1 : seq_extend a'.seq + seq_extend b'.seq = seq_extend (a' + b').seq := by
+      congr
+
+    rw [h1]
+    rw [summationHomeo]
+
+  simp
+  intro d d' dR
+
+  show Param10 (G1 d) (G2 d')
+
+  show Param10 (d = c) (d' = c')
+
+
+  -- Part 4: Relate eq:  X  *=*  X
+  --                        ___
+  --
+  let H1 := fun (f : _ -> _ -> Sort _) => (f d c)
+  let C1 := @Eq xnnR
+
+  let H2 := fun (f : _ -> _ -> Sort _) => (f d' c')
+  let C2 := @Eq nnR
+
+  -- tr_split_application
+
+  -- This and variations do not work
+  -- show Param10 ((. _ _) _ _) ((. _ _) _ _)
+  -- show Param10 ((fun (f : _ -> _ -> Sort _) => f _ _) _) ((fun (f : _ -> _ -> Sort _) => f _ _) _)
+
+  let eqParam : Param00 (xnnR → xnnR → Prop) (nnR → nnR → Prop) := by
+    tr_split'
+    case p1 => infer_instance
+
+    tr_split'
+    case p1 => infer_instance
+
+    -- TODO: Make this work with infer_instance
+    exact propParam.forget
+
+
+    /-
+    Previous approach:
+
+    ```
+    -- Use Prop related to Prop by identity.
+    infer_instance
+    ```
+
+    Approach before that:
+    ```
+    apply Param_from_map
+    intro f x y
+    exact f (.fin x) (.fin y)
+    ```
+    -/
+
+  -- Why can't we simplify the value of a hypothesis? (Only the type)
+  -- simp [inferInstance, eqParam, Param_arrow.Map4_arrow] at eqParam
+
+  show Param10 (H1 C1) (H2 C2)
+  apply forallApplication
+
+  /-
+  Currently, we can't use `tr_split_application` here yet, because the
+  implicit argument gets converted, and also we haven't implemented
+  transferring the function head itself:
+
+  ```plaintext
+  Would relate:    (@Eq.{1} xnnR d c) (@Eq.{1} nnR d' c')
+                            ----               ---
+  ```
+  -/
+
+
+  case p1 =>
+    show Param00 (xnnR → xnnR → Prop) (nnR → nnR → Prop)
+    infer_instance
+
+  case aR =>
+    dsimp [inferInstance, eqParam, Param_arrow.Map1_arrow]
+
+    -- We need to use `propParam` instance for `Param Prop Prop`, not the
+    -- instance defined by equality.
+    unfold propParam
+    unfold C1 C2
+
+    dsimp
+    intro x x' xR
+    intro y y' yR
+
+    show x = y → x' = y'
+
+    have xF := tr.R_implies_map x x' xR
+    have yF := tr.R_implies_map y y' yR
+
+    dsimp at xF yF
+    subst xF yF
+
+    show x = y → tr.map x = tr.map y
+    exact congrArg _
+
+    -- Previous approach:
+    -- -- Since we related Props by id, we have to prove the two Props are equal.
+    -- -- Ideally we would only want to proof the implication. This would be
+    -- -- addressed by implementing translation of the types in the propositions
+    -- -- using registed Param instances.
+    -- show C1 x y = C2 x' y'
+
+    -- unfold C1 C2
+    -- show (x = y) = (x' = y')
+
+    -- apply propext
+
+    -- constructor
+    -- · show (x = y → x' = y')
+    --   have xF := tr.R_implies_map x x' xR
+    --   have yF := tr.R_implies_map y y' yR
+
+    --   dsimp at xF yF
+    --   subst xF yF
+
+    --   intro h
+    --   congr
+
+    -- · show (x' = y' → x = y)
+    --   have xF := tr.R_implies_map x' x xR
+    --   have yF := tr.R_implies_map y' y yR
+
+    --   dsimp at xF yF
+    --   subst xF yF
+
+    --   intro h
+    --   congr
+
+  simp
+  intro e e' eR
+
+  show Param10 (H1 e) (H2 e')
+
+  -- let eF := tr.R_implies_map e e' eR
+  -- dsimp at eF
+
+
+  -- Part 5: Use relations to make the relation trivial
+  --
+  show Param10 (e d c) (e' d' c')
+  dsimp [inferInstance, eqParam, Param_arrow.Map0_arrow, propParam] at eR
+
+  tr_from_map
+  show e d c → e' d' c'
+
+  exact eR d d' dR c c' cR
+
+  -- Previous approach
+  -- tr_ident
+  -- show e d c = e' d' c'
+  -- ...
